src/Predicate.v
@@ -1,0 +1,31 @@
+Require Import Bool List String Peano_dec.
+Require Import Common FMap Syntax Semantics.
+
+Set Implicit Arguments.
+
+Definition OInv := OState (* object state *) -> Value -> Prop.
+Definition Inv := M.t (* object index *) OInv.
+
+Definition InvSat (inv: Inv) (val: Value) (oss: ObjectStates) :=
+  forall oidx oinv,
+    inv@[oidx] = Some oinv ->
+    match oss@[oidx] with
+    | Some os => oinv os val
+    | None => False
+    end.
+
+Record InvO :=
+  { io_idx: IdxT;
+    io_st: OState;
+    io_inv: OInv;
+    io_val: Value;
+    io_sat: io_inv io_st io_val }.
+
+Record InvOs :=
+  { ios_oss: ObjectStates;
+    ios_inv: Inv;
+    ios_val: Value;
+    ios_sat: InvSat ios_inv ios_val ios_oss }.
+
+Definition Pred := Inv.
+
