src/Synthesis.v
@@ -1,6 +1,6 @@
 Require Import Bool List String Peano_dec.
 Require Import Common FMap Syntax Semantics SemFacts.
-Require Import StepDet StepSeq Serial SerialFacts Simulation.
+Require Import StepDet StepSeq Serial SerialFacts Simulation Predicate.
 
 Section SimP.
 
@@ -9,7 +9,7 @@ Section SimP.
     (impl0 spec: System)
     (R: TState -> TState -> Prop)
     (p: Label -> Label).
-  
+
   Definition SynthOk (s: System) :=
     Serial s step_det /\
     R (getStateInit s) (getStateInit spec) /\
@@ -19,8 +19,8 @@ Section SimP.
 
   Section SynthesisStep.
 
-    Variable syn: System -> System -> Prop.
-    Infix "↪" := syn (at level 30).
+    Definition SynT := System -> System -> Prop.
+    Variable syn: SynT.
 
     (** The synthesizer [syn] should "preserve" three conditions:
      * 1) initial state
@@ -57,4 +57,196 @@ Section SimP.
   End SynthesisStep.
 
 End SimP.
+
+Section SynPerObj.
+  Variables (trsIdx: IdxT)
+            (this: IdxT).
+
+  Definition synPMsgOuts (tos: list IdxT) (val: Value) :=
+    map (fun to => {| msg_id := {| mid_type := trsIdx;
+                                   mid_from := this;
+                                   mid_to := to;
+                                   mid_chn := 0; (* TODO: how to decide a channel to use *)
+                                |};
+                      msg_value := val
+                   |}) tos.
+
+  Section Request.
+    Variables (rqfrom: IdxT) (fwds: list IdxT).
+
+    (* TODO: correct preconditions for safe interleavings *)
+    Definition synPMsgRqPrecond (st: OState) := True.
+
+    Definition synPMsgRqPostcond (pre: OState) (val: Value) (post: OState) :=
+      post = {| ost_st := ost_st pre;
+                ost_tst := (ost_tst pre)
+                           +[ trsIdx <- {| tst_rqfrom := rqfrom;
+                                           tst_rqfwds := map (fun idx => (idx, false)) fwds |}]
+             |}.
+
+    Definition synPMsgRq (chn: IdxT): PMsg :=
+      {| pmsg_mid := {| mid_type := trsIdx;
+                        mid_from := rqfrom;
+                        mid_to := this;
+                        mid_chn := chn |};
+         pmsg_precond := synPMsgRqPrecond;
+         pmsg_outs := fun _ val => synPMsgOuts fwds val;
+         pmsg_postcond := synPMsgRqPostcond |}.
+
+  End Request.
+
+  Section Response.
+    Variable rsFrom: IdxT.
+
+    (* TODO: pre/postconditions for safe interleavings *)
+    Definition synPMsgRsPrecond (st: OState) :=
+      True.
+
+    Fixpoint addResponse (fwds: list (IdxT * bool)) :=
+      match fwds with
+      | nil => nil
+      | (idx, b) :: fwds' =>
+        if idx ==n rsFrom
+        then (idx, true) :: fwds'
+        else (idx, b) :: (addResponse fwds')
+      end.
+
+    Definition Responded (pre: OState) (post: OState) :=
+      (ost_tst pre)@[trsIdx] >>=[False]
+      (fun preth =>
+         (ost_tst post)@[trsIdx] >>=[False]
+         (fun postth =>
+            postth = {| tst_rqfrom := tst_rqfrom preth;
+                        tst_rqfwds := addResponse (tst_rqfwds preth) |})).
+
+    Definition allResponded (fwds: list (IdxT * bool)) :=
+      forallb (fun ib => snd ib) fwds.
+
+    Definition WhenAllResponded (oinv: OInv) (val: Value)
+               (pre post: OState) :=
+      (ost_tst post)@[trsIdx] >>=[False]
+      (fun trsh =>
+         if allResponded (tst_rqfwds trsh)
+         then pre = post
+         else oinv post val).
+
+    Definition synPMsgRsPostcond (oinv: OInv) (pre: OState) (val: Value) (post: OState) :=
+      Responded pre post /\
+      WhenAllResponded oinv val pre post.
+
+    (* TODO: how to decide a channel [chn] to use *)
+    Definition synPMsgRs (chn: IdxT) (oinv: OInv): PMsg :=
+      {| pmsg_mid := {| mid_type := trsIdx;
+                        mid_from := rsFrom;
+                        mid_to := this;
+                        mid_chn := chn |};
+         pmsg_precond := synPMsgRsPrecond;
+         pmsg_outs :=
+           fun st val =>
+             (ost_tst st)@[trsIdx] >>=[nil]
+             (fun trsh =>
+                if allResponded (tst_rqfwds trsh)
+                then synPMsgOuts (tst_rqfrom trsh :: nil) val
+                else nil);
+         pmsg_postcond := synPMsgRsPostcond oinv |}.
+
+    Definition synPMsgImm (chn: IdxT) (oinv: OInv): PMsg :=
+      {| pmsg_mid := {| mid_type := trsIdx;
+                        mid_from := rsFrom;
+                        mid_to := this;
+                        mid_chn := chn |};
+         pmsg_precond := fun _ => True;
+         pmsg_outs := fun _ val => synPMsgOuts (rsFrom :: nil) val;
+         pmsg_postcond := synPMsgRsPostcond oinv |}.
+
+  End Response.
+  
+End SynPerObj.
+
+Section SynPerTrs.
+
+  Variables
+    (* A transaction index uniquely assigned for this transaction *)
+    (trsIdx: IdxT)
+    (trsVal: Value)
+    (* A transaction predicate *)
+    (trspred: Pred).
+
+  Local Definition targetObjs := map fst (M.elements trspred).
+
+  Fixpoint getTos (me: IdxT) (topo: list Channel) :=
+    match topo with
+    | nil => nil
+    | chn :: t =>
+      if me ==n chn_from chn
+      then chn_to chn :: getTos me t
+      else getTos me t
+    end.
+
+  Fixpoint idxInter (li1 li2: list IdxT) :=
+    filter (fun idx => if idx ?<n li2 then true else false) li1.
+
+  Inductive SynTrs (efrom hdl: IdxT) (topo: list Channel):
+    list MsgId (* currently synthesizable messages *) ->
+    Pred (* current transaction predicate *) ->
+    list Object (* synthesized objects *) -> Prop :=
+  | SynTrsStart:
+      forall objs chn mid,
+        mid = {| mid_type := trsIdx; mid_from := efrom; mid_to := hdl; mid_chn := chn |} ->
+        SynTrs efrom hdl topo (mid :: nil) trspred objs
+  | SynTrsStep:
+      forall oidx mids1 mid mids2 preds objs1 obj objs2 oinv fwds synrq synrss mouts nobj,
+        SynTrs efrom hdl topo (mids1 ++ mid :: mids2) preds (objs1 ++ obj :: objs2) ->
+        oidx = mid_to mid ->
+        oidx = obj_idx obj ->
+        preds@[oidx] = Some oinv ->
+        fwds = idxInter (getTos oidx topo) targetObjs ->
+        synrq = synPMsgRq trsIdx oidx (mid_from mid) fwds (mid_chn mid) ->
+        synrss = map (fun ridx =>
+                        synPMsgRs trsIdx oidx ridx O (* TODO: channel... *)
+                                  oinv
+                     )
+                     fwds ->
+        mouts = synPMsgOuts oidx trsIdx
+                            (idxInter (getTos oidx topo) targetObjs)
+                            trsVal ->
+        nobj = {| obj_idx := obj_idx obj;
+                  obj_state_init := obj_state_init obj;
+                  obj_trs := synrq :: synrss ++ obj_trs obj |} ->
+        forall nmids npreds nobjs,
+          nmids = mids1 ++ mids2 ++ map msg_id mouts ->
+          npreds = M.remove oidx preds ->
+          nobjs = objs1 ++ nobj :: objs2 ->
+          SynTrs efrom hdl topo nmids npreds nobjs
+  | SynTrsEnd:
+      forall oidx mids1 mid mids2 preds objs1 obj objs2 oinv synimm nobj,
+        SynTrs efrom hdl topo (mids1 ++ mid :: mids2) preds (objs1 ++ obj :: objs2) ->
+        oidx = mid_to mid ->
+        oidx = obj_idx obj ->
+        preds@[oidx] = Some oinv ->
+        idxInter (getTos oidx topo) targetObjs = nil ->
+        synimm = synPMsgImm trsIdx oidx (mid_from mid) (mid_chn mid) oinv ->
+        nobj = {| obj_idx := obj_idx obj;
+                  obj_state_init := obj_state_init obj;
+                  obj_trs := synimm :: obj_trs obj |} ->
+        forall nmids npreds nobjs,
+          nmids = mids1 ++ mids2 ->
+          npreds = M.remove oidx preds ->
+          nobjs = objs1 ++ nobj :: objs2 ->
+          SynTrs efrom hdl topo nmids npreds nobjs.
+
+  Definition SynTrsFinished (efrom hdl: IdxT) (topo: list Channel) (objs: list Object) :=
+    SynTrs efrom hdl topo nil (M.empty _) objs.
+
+End SynPerTrs.
+
+Section Synthesizer.
+
+  (* A target system *)
+  Variable sys: System.
+
+  Local Definition objs := sys_objs sys.
+  Local Definition topo := sys_chns sys.
+
+End Synthesizer.
 
